chore(library/init): move logic.lean => core.lean

library/init/core.lean
@@ -45,7 +45,7 @@ reserve infixl ` % `:70
 reserve prefix `-`:100
 reserve infixr ` ^ `:80
 
-reserve infixr ` ∘ `:90                 -- input with \comp
+reserve infixr ` ∘ `:90
 
 reserve infix ` <= `:50
 reserve infix ` ≤ `:50
@@ -80,6 +80,11 @@ reserve infixr ` :: `:67
 reserve infixl `; `:1
 
 universes u v w
+
+@[inline] def id {α : Sort u} (a : α) : α := a
+
+@[inline] def flip {α : Sort u} {β : Sort v} {φ : Sort w} (f : α → β → φ) : β → α → φ :=
+λ b a, f a b
 
 /-
 The kernel definitional equality test (t =?= s) has special support for id_delta applications.
@@ -182,6 +187,9 @@ def and.elim_left {a b : Prop} (h : and a b) : a := h.1
 
 def and.elim_right {a b : Prop} (h : and a b) : b := h.2
 
+structure iff (a b : Prop) : Prop :=
+intro :: (mp : a → b) (mpr : b → a)
+
 /- eq basic support -/
 
 infix = := eq
@@ -191,22 +199,22 @@ attribute [refl] eq.refl
 @[pattern] def rfl {α : Sort u} {a : α} : a = a := eq.refl a
 
 @[elab_as_eliminator, subst]
-lemma eq.subst {α : Sort u} {P : α → Prop} {a b : α} (h₁ : a = b) (h₂ : P a) : P b :=
+theorem eq.subst {α : Sort u} {P : α → Prop} {a b : α} (h₁ : a = b) (h₂ : P a) : P b :=
 eq.rec h₂ h₁
 
 notation h1 ▸ h2 := eq.subst h1 h2
 
-@[trans] lemma eq.trans {α : Sort u} {a b c : α} (h₁ : a = b) (h₂ : b = c) : a = c :=
+@[trans] theorem eq.trans {α : Sort u} {a b c : α} (h₁ : a = b) (h₂ : b = c) : a = c :=
 h₂ ▸ h₁
 
-@[symm] lemma eq.symm {α : Sort u} {a b : α} (h : a = b) : b = a :=
+@[symm] theorem eq.symm {α : Sort u} {a b : α} (h : a = b) : b = a :=
 h ▸ rfl
 
 infix == := heq
 
 @[pattern] def heq.rfl {α : Sort u} {a : α} : a == a := heq.refl a
 
-lemma eq_of_heq {α : Sort u} {a a' : α} (h : a == a') : a = a' :=
+theorem eq_of_heq {α : Sort u} {a a' : α} (h : a == a') : a = a' :=
 have ∀ (α' : Sort u) (a' : α') (h₁ : @heq α a α' a') (h₂ : α = α'), (eq.rec_on h₂ a : α') = a', from
   λ (α' : Sort u) (a' : α') (h₁ : @heq α a α' a'), heq.rec_on h₁ (λ h₂ : α = α, rfl),
 show (eq.rec_on (eq.refl α) a : α) = a', from
@@ -214,19 +222,19 @@ show (eq.rec_on (eq.refl α) a : α) = a', from
 
 /- The following four lemmas could not be automatically generated when the
    structures were declared, so we prove them manually here. -/
-lemma prod.mk.inj {α : Type u} {β : Type v} {x₁ : α} {y₁ : β} {x₂ : α} {y₂ : β}
+theorem prod.mk.inj {α : Type u} {β : Type v} {x₁ : α} {y₁ : β} {x₂ : α} {y₂ : β}
   : (x₁, y₁) = (x₂, y₂) → and (x₁ = x₂) (y₁ = y₂) :=
 λ h, prod.no_confusion h (λ h₁ h₂, ⟨h₁, h₂⟩)
 
-lemma prod.mk.inj_arrow {α : Type u} {β : Type v} {x₁ : α} {y₁ : β} {x₂ : α} {y₂ : β}
+theorem prod.mk.inj_arrow {α : Type u} {β : Type v} {x₁ : α} {y₁ : β} {x₂ : α} {y₂ : β}
   : (x₁, y₁) = (x₂, y₂) → Π ⦃P : Sort w⦄, (x₁ = x₂ → y₁ = y₂ → P) → P :=
 λ h₁ _ h₂, prod.no_confusion h₁ h₂
 
-lemma pprod.mk.inj {α : Sort u} {β : Sort v} {x₁ : α} {y₁ : β} {x₂ : α} {y₂ : β}
+theorem pprod.mk.inj {α : Sort u} {β : Sort v} {x₁ : α} {y₁ : β} {x₂ : α} {y₂ : β}
   : pprod.mk x₁ y₁ = pprod.mk x₂ y₂ → and (x₁ = x₂) (y₁ = y₂) :=
 λ h, pprod.no_confusion h (λ h₁ h₂, ⟨h₁, h₂⟩)
 
-lemma pprod.mk.inj_arrow {α : Type u} {β : Type v} {x₁ : α} {y₁ : β} {x₂ : α} {y₂ : β}
+theorem pprod.mk.inj_arrow {α : Type u} {β : Type v} {x₁ : α} {y₁ : β} {x₂ : α} {y₂ : β}
   : (x₁, y₁) = (x₂, y₂) → Π ⦃P : Sort w⦄, (x₁ = x₂ → y₁ = y₂ → P) → P :=
 λ h₁ _ h₂, prod.no_confusion h₁ h₂
 
@@ -261,6 +269,12 @@ inductive bool : Type
 /- Remark: subtype must take a Sort instead of Type because of the axiom strong_indefinite_description. -/
 structure subtype {α : Sort u} (p : α → Prop) :=
 (val : α) (property : p val)
+
+inductive Exists {α : Sort u} (p : α → Prop) : Prop
+| intro (w : α) (h : p w) : Exists
+
+def exists_unique {α : Sort u} (p : α → Prop) :=
+Exists (λ x, and (p x) (∀ y, p y → y = x))
 
 attribute [pp_using_anonymous_constructor] sigma psigma subtype pprod and
 
@@ -359,6 +373,15 @@ infix ⊂        := has_ssubset.ssubset
 infix \        := has_sdiff.sdiff
 infix ≈        := has_equiv.equiv
 infixr ^       := has_pow.pow
+infixr /\      := and
+infixr ∧       := and
+infixr \/      := or
+infixr ∨       := or
+infix <->      := iff
+infix ↔        := iff
+notation `exists` binders `, ` r:(scoped P, Exists P) := r
+notation `∃` binders `, ` r:(scoped P, Exists P) := r
+notation `∃!` binders `, ` r:(scoped P, exists_unique P) := r
 
 export has_append (append)
 
@@ -388,16 +411,13 @@ def singleton {α : Type u} {γ : Type v} [has_emptyc γ] [has_insert α γ] (a 
 has_insert.insert a ∅
 
 /- nat basic instances -/
+protected def nat.add : nat → nat → nat
+| a  nat.zero     := a
+| a  (nat.succ b) := nat.succ (nat.add a b)
 
-namespace nat
-  protected def add : nat → nat → nat
-  | a  zero     := a
-  | a  (succ b) := succ (add a b)
-
-  /- We mark the following definitions as pattern to make sure they can be used in recursive equations,
-     and reduced by the equation compiler. -/
-  attribute [pattern] nat.add nat.add._main
-end nat
+/- We mark the following definitions as pattern to make sure they can be used in recursive equations,
+   and reduced by the equation compiler. -/
+attribute [pattern] nat.add nat.add._main
 
 instance : has_zero nat := ⟨nat.zero⟩
 
@@ -408,9 +428,7 @@ instance : has_add nat := ⟨nat.add⟩
 def std.priority.default : nat := 1000
 def std.priority.max     : nat := 0xFFFFFFFF
 
-namespace nat
-  protected def prio := std.priority.default + 100
-end nat
+protected def nat.prio := std.priority.default + 100
 
 /-
   Global declarations of right binding strength
@@ -524,7 +542,7 @@ protected def subtype.sizeof {α : Type u} [has_sizeof α] {p : α → Prop} : s
 instance {α : Type u} [has_sizeof α] (p : α → Prop) : has_sizeof (subtype p) :=
 ⟨subtype.sizeof⟩
 
-lemma nat_add_zero (n : nat) : n + 0 = n := rfl
+theorem nat_add_zero (n : nat) : n + 0 = n := rfl
 
 /- Combinator calculus -/
 namespace combinator
@@ -533,6 +551,8 @@ def I {α : Type u₁} (a : α) := a
 def K {α : Type u₁} {β : Type u₂} (a : α) (b : β) := a
 def S {α : Type u₁} {β : Type u₂} {γ : Type u₃} (x : α → β → γ) (y : α → β) (z : α) := x z (y z)
 end combinator
+
+@[simp] theorem opt_param_eq (α : Sort u) (default : α) : opt_param α default = α := rfl
 
 /-- Auxiliary datatype for #[ ... ] notation.
     #[1, 2, 3, 4] is notation for
@@ -583,16 +603,827 @@ notation !x     := bnot x
 notation x || y := bor x y
 notation x && y := band x y
 
+/- Logical connectives an equality -/
+
+def implies (a b : Prop) := a → b
+
+@[trans] theorem implies.trans {p q r : Prop} (h₁ : implies p q) (h₂ : implies q r) : implies p r :=
+assume hp, h₂ (h₁ hp)
+
+def trivial : true := ⟨⟩
+
+@[inline] def absurd {a : Prop} {b : Sort v} (h₁ : a) (h₂ : ¬a) : b :=
+false.rec b (h₂ h₁)
+
+theorem mt {a b : Prop} (h₁ : a → b) (h₂ : ¬b) : ¬a := assume ha : a, h₂ (h₁ ha)
+
+theorem not.intro {a : Prop} (h : a → false) : ¬ a := h
+
+theorem not_false : ¬false := id
+
+@[inline] def false.elim {C : Sort u} (h : false) : C :=
+false.rec C h
+
+-- proof irrelevance is built in
+theorem proof_irrel {a : Prop} (h₁ h₂ : a) : h₁ = h₂ := rfl
+
+@[simp] theorem id.def {α : Sort u} (a : α) : id a = a := rfl
+
+@[inline] def eq.mp {α β : Sort u} (h₁ : α = β) (h₂ : α) : β :=
+eq.rec_on h₁ h₂
+
+@[inline] def eq.mpr {α β : Sort u} : (α = β) → β → α :=
+λ h₁ h₂, eq.rec_on (eq.symm h₁) h₂
+
+@[elab_as_eliminator]
+theorem eq.substr {α : Sort u} {p : α → Prop} {a b : α} (h₁ : b = a) (h₂ : p a) : p b :=
+eq.subst (eq.symm h₁) h₂
+
+theorem congr {α : Sort u} {β : Sort v} {f₁ f₂ : α → β} {a₁ a₂ : α} (h₁ : f₁ = f₂) (h₂ : a₁ = a₂) : f₁ a₁ = f₂ a₂ :=
+eq.subst h₁ (eq.subst h₂ rfl)
+
+theorem congr_fun {α : Sort u} {β : α → Sort v} {f g : Π x, β x} (h : f = g) (a : α) : f a = g a :=
+eq.subst h (eq.refl (f a))
+
+theorem congr_arg {α : Sort u} {β : Sort v} {a₁ a₂ : α} (f : α → β) (h : a₁ = a₂) : f a₁ = f a₂ :=
+congr rfl h
+
+theorem trans_rel_left {α : Sort u} {a b c : α} (r : α → α → Prop) (h₁ : r a b) (h₂ : b = c) : r a c :=
+h₂ ▸ h₁
+
+theorem trans_rel_right {α : Sort u} {a b c : α} (r : α → α → Prop) (h₁ : a = b) (h₂ : r b c) : r a c :=
+h₁.symm ▸ h₂
+
+theorem of_eq_true {p : Prop} (h : p = true) : p :=
+h.symm ▸ trivial
+
+theorem not_of_eq_false {p : Prop} (h : p = false) : ¬p :=
+assume hp, h ▸ hp
+
+@[inline] def cast {α β : Sort u} (h : α = β) (a : α) : β :=
+eq.rec a h
+
+theorem cast_proof_irrel {α β : Sort u} (h₁ h₂ : α = β) (a : α) : cast h₁ a = cast h₂ a := rfl
+
+theorem cast_eq {α : Sort u} (h : α = α) (a : α) : cast h a = a := rfl
+
+@[reducible] def ne {α : Sort u} (a b : α) := ¬(a = b)
+notation a ≠ b := ne a b
+
+@[simp] theorem ne.def {α : Sort u} (a b : α) : a ≠ b = ¬ (a = b) := rfl
+
+section ne
+variable {α : Sort u}
+variables {a b : α} {p : Prop}
+
+theorem ne.intro (h : a = b → false) : a ≠ b := h
+
+theorem ne.elim (h : a ≠ b) : a = b → false := h
+
+theorem ne.irrefl (h : a ≠ a) : false := h rfl
+
+theorem ne.symm (h : a ≠ b) : b ≠ a :=
+assume (h₁ : b = a), h (h₁.symm)
+
+theorem false_of_ne : a ≠ a → false := ne.irrefl
+
+theorem ne_false_of_self : p → p ≠ false :=
+assume (hp : p) (heq : p = false), heq ▸ hp
+
+theorem ne_true_of_not : ¬p → p ≠ true :=
+assume (hnp : ¬p) (heq : p = true), (heq ▸ hnp) trivial
+
+theorem true_ne_false : ¬true = false :=
+ne_false_of_self trivial
+end ne
+
+attribute [refl] heq.refl
+
+section
+variables {α β φ : Sort u} {a a' : α} {b b' : β} {c : φ}
+
+theorem heq.elim {α : Sort u} {a : α} {p : α → Sort v} {b : α} (h₁ : a == b) (h₂ : p a) : p b :=
+eq.rec_on (eq_of_heq h₁) h₂
+
+theorem heq.subst {p : ∀ T : Sort u, T → Prop} (h₁ : a == b) (h₂ : p α a) : p β b :=
+heq.rec_on h₁ h₂
+
+@[symm] theorem heq.symm (h : a == b) : b == a :=
+heq.rec_on h (heq.refl a)
+
+theorem heq_of_eq (h : a = a') : a == a' :=
+eq.subst h (heq.refl a)
+
+@[trans] theorem heq.trans (h₁ : a == b) (h₂ : b == c) : a == c :=
+heq.subst h₂ h₁
+
+@[trans] theorem heq_of_heq_of_eq (h₁ : a == b) (h₂ : b = b') : a == b' :=
+heq.trans h₁ (heq_of_eq h₂)
+
+@[trans] theorem heq_of_eq_of_heq (h₁ : a = a') (h₂ : a' == b) : a == b :=
+heq.trans (heq_of_eq h₁) h₂
+
+def type_eq_of_heq (h : a == b) : α = β :=
+heq.rec_on h (eq.refl α)
+end
+
+theorem eq_rec_heq {α : Sort u} {φ : α → Sort v} : ∀ {a a' : α} (h : a = a') (p : φ a), (eq.rec_on h p : φ a') == p
+| a _ rfl p := heq.refl p
+
+theorem heq_of_eq_rec_left {α : Sort u} {φ : α → Sort v} : ∀ {a a' : α} {p₁ : φ a} {p₂ : φ a'} (e : a = a') (h₂ : (eq.rec_on e p₁ : φ a') = p₂), p₁ == p₂
+| a _ p₁ p₂ rfl h := eq.rec_on h (heq.refl p₁)
+
+theorem heq_of_eq_rec_right {α : Sort u} {φ : α → Sort v} : ∀ {a a' : α} {p₁ : φ a} {p₂ : φ a'} (e : a' = a) (h₂ : p₁ = eq.rec_on e p₂), p₁ == p₂
+| a _ p₁ p₂ rfl h :=
+  have p₁ = p₂, from h,
+  this ▸ heq.refl p₁
+
+theorem of_heq_true {a : Prop} (h : a == true) : a :=
+of_eq_true (eq_of_heq h)
+
+theorem eq_rec_compose : ∀ {α β φ : Sort u} (p₁ : β = φ) (p₂ : α = β) (a : α), (eq.rec_on p₁ (eq.rec_on p₂ a : β) : φ) = eq.rec_on (eq.trans p₂ p₁) a
+| α _ _ rfl rfl a := rfl
+
+theorem cast_heq : ∀ {α β : Sort u} (h : α = β) (a : α), cast h a == a
+| α _ rfl a := heq.refl a
+
+variables {a b c d : Prop}
+
+theorem and.elim (h₁ : a ∧ b) (h₂ : a → b → c) : c :=
+and.rec h₂ h₁
+
+theorem and.swap : a ∧ b → b ∧ a :=
+assume ⟨ha, hb⟩, ⟨hb, ha⟩
+
+def and.symm := @and.swap
+
+theorem or.elim (h₁ : a ∨ b) (h₂ : a → c) (h₃ : b → c) : c :=
+or.rec h₂ h₃ h₁
+
+theorem non_contradictory_em (a : Prop) : ¬¬(a ∨ ¬a) :=
+assume not_em : ¬(a ∨ ¬a),
+  have neg_a : ¬a, from
+    assume pos_a : a, absurd (or.inl pos_a) not_em,
+  absurd (or.inr neg_a) not_em
+
+def not_not_em := non_contradictory_em
+
+theorem or.swap : a ∨ b → b ∨ a := or.rec or.inr or.inl
+
+def or.symm := @or.swap
+
+/- xor -/
+def xor (a b : Prop) := (a ∧ ¬ b) ∨ (b ∧ ¬ a)
+
+@[recursor 5]
+theorem iff.elim : ((a → b) → (b → a) → c) → (a ↔ b) → c := iff.rec
+
+theorem iff.elim_left : (a ↔ b) → a → b := iff.mp
+
+theorem iff.elim_right : (a ↔ b) → b → a := iff.mpr
+
+theorem iff_iff_implies_and_implies (a b : Prop) : (a ↔ b) ↔ (a → b) ∧ (b → a) :=
+iff.intro (λ h, and.intro h.mp h.mpr) (λ h, iff.intro h.left h.right)
+
+@[refl]
+theorem iff.refl (a : Prop) : a ↔ a :=
+iff.intro (assume h, h) (assume h, h)
+
+theorem iff.rfl {a : Prop} : a ↔ a :=
+iff.refl a
+
+@[trans]
+theorem iff.trans (h₁ : a ↔ b) (h₂ : b ↔ c) : a ↔ c :=
+iff.intro
+  (assume ha, iff.mp h₂ (iff.mp h₁ ha))
+  (assume hc, iff.mpr h₁ (iff.mpr h₂ hc))
+
+@[symm]
+theorem iff.symm (h : a ↔ b) : b ↔ a :=
+iff.intro (iff.elim_right h) (iff.elim_left h)
+
+theorem iff.comm : (a ↔ b) ↔ (b ↔ a) :=
+iff.intro iff.symm iff.symm
+
+theorem eq.to_iff {a b : Prop} (h : a = b) : a ↔ b :=
+eq.rec_on h iff.rfl
+
+theorem neq_of_not_iff {a b : Prop} : ¬(a ↔ b) → a ≠ b :=
+λ h₁ h₂,
+have a ↔ b, from eq.subst h₂ (iff.refl a),
+absurd this h₁
+
+theorem not_iff_not_of_iff (h₁ : a ↔ b) : ¬a ↔ ¬b :=
+iff.intro
+ (assume (hna : ¬ a) (hb : b), hna (iff.elim_right h₁ hb))
+ (assume (hnb : ¬ b) (ha : a), hnb (iff.elim_left h₁ ha))
+
+theorem of_iff_true (h : a ↔ true) : a :=
+iff.mp (iff.symm h) trivial
+
+theorem not_of_iff_false : (a ↔ false) → ¬a := iff.mp
+
+theorem iff_true_intro (h : a) : a ↔ true :=
+iff.intro
+  (λ hl, trivial)
+  (λ hr, h)
+
+theorem iff_false_intro (h : ¬a) : a ↔ false :=
+iff.intro h (false.rec a)
+
+theorem imp_congr (h₁ : a ↔ c) (h₂ : b ↔ d) : (a → b) ↔ (c → d) :=
+iff.intro
+  (λ hab hc, iff.mp h₂ (hab (iff.mpr h₁ hc)))
+  (λ hcd ha, iff.mpr h₂ (hcd (iff.mp h₁ ha)))
+
+theorem imp_congr_ctx (h₁ : a ↔ c) (h₂ : c → (b ↔ d)) : (a → b) ↔ (c → d) :=
+iff.intro
+  (λ hab hc, have ha : a, from iff.mpr h₁ hc,
+             have hb : b, from hab ha,
+             iff.mp (h₂ hc) hb)
+  (λ hcd ha, have hc : c, from iff.mp h₁ ha,
+             have hd : d, from hcd hc,
+iff.mpr (h₂ hc) hd)
+
+theorem imp_congr_right (h : a → (b ↔ c)) : (a → b) ↔ (a → c) :=
+iff.intro
+  (assume hab ha, iff.elim_left (h ha) (hab ha))
+  (assume hab ha, iff.elim_right (h ha) (hab ha))
+
+theorem not_not_intro (ha : a) : ¬¬a :=
+assume hna : ¬a, hna ha
+
+theorem not_of_not_not_not (h : ¬¬¬a) : ¬a :=
+λ ha, absurd (not_not_intro ha) h
+
+@[simp] theorem not_true : (¬ true) ↔ false :=
+iff_false_intro (not_not_intro trivial)
+
+def not_true_iff := not_true
+
+@[simp] theorem not_false_iff : (¬ false) ↔ true :=
+iff_true_intro not_false
+
+@[congr] theorem not_congr (h : a ↔ b) : ¬a ↔ ¬b :=
+iff.intro (λ h₁ h₂, h₁ (iff.mpr h h₂)) (λ h₁ h₂, h₁ (iff.mp h h₂))
+
+@[simp] theorem ne_self_iff_false {α : Sort u} (a : α) : (not (a = a)) ↔ false :=
+iff.intro false_of_ne false.elim
+
+@[simp] theorem eq_self_iff_true {α : Sort u} (a : α) : (a = a) ↔ true :=
+iff_true_intro rfl
+
+@[simp] theorem heq_self_iff_true {α : Sort u} (a : α) : (a == a) ↔ true :=
+iff_true_intro (heq.refl a)
+
+@[simp] theorem iff_not_self (a : Prop) : (a ↔ ¬a) ↔ false :=
+iff_false_intro (λ h,
+   have h' : ¬a, from (λ ha, (iff.mp h ha) ha),
+   h' (iff.mpr h h'))
+
+@[simp] theorem not_iff_self (a : Prop) : (¬a ↔ a) ↔ false :=
+iff_false_intro (λ h,
+   have h' : ¬a, from (λ ha, (iff.mpr h ha) ha),
+   h' (iff.mp h h'))
+
+@[simp] theorem true_iff_false : (true ↔ false) ↔ false :=
+iff_false_intro (λ h, iff.mp h trivial)
+
+@[simp] theorem false_iff_true : (false ↔ true) ↔ false :=
+iff_false_intro (λ h, iff.mpr h trivial)
+
+theorem false_of_true_iff_false : (true ↔ false) → false :=
+assume h, iff.mp h trivial
+
+theorem false_of_true_eq_false : (true = false) → false :=
+assume h, h ▸ trivial
+
+theorem true_eq_false_of_false : false → (true = false) :=
+false.elim
+
+theorem eq_comm {α : Sort u} {a b : α} : a = b ↔ b = a :=
+⟨eq.symm, eq.symm⟩
+
+/- and simp rules -/
+theorem and.imp (hac : a → c) (hbd : b → d) : a ∧ b → c ∧ d :=
+assume ⟨ha, hb⟩, ⟨hac ha, hbd hb⟩
+
+def and_implies := @and.imp
+
+@[congr] theorem and_congr (h₁ : a ↔ c) (h₂ : b ↔ d) : (a ∧ b) ↔ (c ∧ d) :=
+iff.intro (and.imp (iff.mp h₁) (iff.mp h₂)) (and.imp (iff.mpr h₁) (iff.mpr h₂))
+
+theorem and_comm : a ∧ b ↔ b ∧ a :=
+iff.intro and.swap and.swap
+
+theorem and_assoc : (a ∧ b) ∧ c ↔ a ∧ (b ∧ c) :=
+iff.intro
+  (assume ⟨⟨ha, hb⟩, hc⟩, ⟨ha, ⟨hb, hc⟩⟩)
+  (assume ⟨ha, ⟨hb, hc⟩⟩, ⟨⟨ha, hb⟩, hc⟩)
+
+theorem and_left_comm : a ∧ (b ∧ c) ↔ b ∧ (a ∧ c) :=
+iff.trans (iff.symm and_assoc) (iff.trans (and_congr and_comm (iff.refl c)) and_assoc)
+
+@[simp] theorem and_true (a : Prop) : a ∧ true ↔ a :=
+iff.intro and.left (λ ha, ⟨ha, trivial⟩)
+
+@[simp] theorem true_and (a : Prop) : true ∧ a ↔ a :=
+iff.intro and.right (λ h, ⟨trivial, h⟩)
+
+@[simp] theorem and_false (a : Prop) : a ∧ false ↔ false :=
+iff_false_intro and.right
+
+@[simp] theorem false_and (a : Prop) : false ∧ a ↔ false :=
+iff_false_intro and.left
+
+@[simp] theorem not_and_self (a : Prop) : (¬a ∧ a) ↔ false :=
+iff_false_intro (λ h, and.elim h (λ h₁ h₂, absurd h₂ h₁))
+
+@[simp] theorem and_not_self (a : Prop) : (a ∧ ¬a) ↔ false :=
+iff_false_intro (assume ⟨h₁, h₂⟩, absurd h₁ h₂)
+
+@[simp] theorem and_self (a : Prop) : a ∧ a ↔ a :=
+iff.intro and.left (assume h, ⟨h, h⟩)
+
+/- or simp rules -/
+
+@[congr] theorem or_congr (h₁ : a ↔ c) (h₂ : b ↔ d) : (a ∨ b) ↔ (c ∨ d) :=
+iff.intro (λ h, or.elim h (λ h, or.inl (iff.mp h₁ h)) (λ h, or.inr (iff.mp h₂ h)))
+          (λ h, or.elim h (λ h, or.inl (iff.mpr h₁ h)) (λ h, or.inr (iff.mpr h₂ h)))
+
+theorem or_comm : a ∨ b ↔ b ∨ a := iff.intro or.swap or.swap
+
+theorem or_assoc : (a ∨ b) ∨ c ↔ a ∨ (b ∨ c) :=
+iff.intro (λ h, or.elim h (λ h, or.elim h or.inl (λ h, or.inr (or.inl h))) (λ h, or.inr (or.inr h)))
+          (λ h, or.elim h (λ h, or.inl (or.inl h)) (λ h, or.elim h (λ h, or.inl (or.inr h)) or.inr))
+
+theorem or_left_comm : a ∨ (b ∨ c) ↔ b ∨ (a ∨ c) :=
+iff.trans (iff.symm or_assoc) (iff.trans (or_congr or_comm (iff.refl c)) or_assoc)
+
+@[simp] theorem or_true (a : Prop) : a ∨ true ↔ true :=
+iff_true_intro (or.inr trivial)
+
+@[simp] theorem true_or (a : Prop) : true ∨ a ↔ true :=
+iff_true_intro (or.inl trivial)
+
+@[simp] theorem or_false (a : Prop) : a ∨ false ↔ a :=
+iff.intro (or.rec id false.elim) or.inl
+
+@[simp] theorem false_or (a : Prop) : false ∨ a ↔ a :=
+iff.trans or_comm (or_false a)
+
+@[simp] theorem or_self (a : Prop) : a ∨ a ↔ a :=
+iff.intro (or.rec id id) or.inl
+
+theorem not_or {a b : Prop} : ¬ a → ¬ b → ¬ (a ∨ b)
+| hna hnb (or.inl ha) := absurd ha hna
+| hna hnb (or.inr hb) := absurd hb hnb
+
+/- or resolution rulses -/
+
+def resolve_left {a b : Prop} (h : a ∨ b) (na : ¬ a) : b :=
+or.elim h (λ ha, absurd ha na) id
+
+def neg_resolve_left {a b : Prop} (h : ¬ a ∨ b) (ha : a) : b :=
+or.elim h (λ na, absurd ha na) id
+
+def resolve_right {a b : Prop} (h : a ∨ b) (nb : ¬ b) : a :=
+or.elim h id (λ hb, absurd hb nb)
+
+def neg_resolve_right {a b : Prop} (h : a ∨ ¬ b) (hb : b) : a :=
+or.elim h id (λ nb, absurd hb nb)
+
+/- iff simp rules -/
+
+@[simp] theorem iff_true (a : Prop) : (a ↔ true) ↔ a :=
+iff.intro (assume h, iff.mpr h trivial) iff_true_intro
+
+@[simp] theorem true_iff (a : Prop) : (true ↔ a) ↔ a :=
+iff.trans iff.comm (iff_true a)
+
+@[simp] theorem iff_false (a : Prop) : (a ↔ false) ↔ ¬ a :=
+iff.intro iff.mp iff_false_intro
+
+@[simp] theorem false_iff (a : Prop) : (false ↔ a) ↔ ¬ a :=
+iff.trans iff.comm (iff_false a)
+
+@[simp] theorem iff_self (a : Prop) : (a ↔ a) ↔ true :=
+iff_true_intro iff.rfl
+
+@[congr] theorem iff_congr (h₁ : a ↔ c) (h₂ : b ↔ d) : (a ↔ b) ↔ (c ↔ d) :=
+(iff_iff_implies_and_implies a b).trans
+  ((and_congr (imp_congr h₁ h₂) (imp_congr h₂ h₁)).trans
+    (iff_iff_implies_and_implies c d).symm)
+
+/- implies simp rule -/
+@[simp] theorem implies_true_iff (α : Sort u) : (α → true) ↔ true :=
+iff.intro (λ h, trivial) (λ ha h, trivial)
+
+@[simp] theorem false_implies_iff (a : Prop) : (false → a) ↔ true :=
+iff.intro (λ h, trivial) (λ ha h, false.elim h)
+
+@[simp] theorem true_implies_iff (α : Prop) : (true → α) ↔ α :=
+iff.intro (λ h, h trivial) (λ h h', h)
+
+/- exists -/
+
+@[pattern]
+def exists.intro := @Exists.intro
+
+theorem exists.elim {α : Sort u} {p : α → Prop} {b : Prop}
+  (h₁ : ∃ x, p x) (h₂ : ∀ (a : α), p a → b) : b :=
+Exists.rec h₂ h₁
+
+/- exists unique -/
+
+theorem exists_unique.intro {α : Sort u} {p : α → Prop} (w : α) (h₁ : p w) (h₂ : ∀ y, p y → y = w) :
+  ∃! x, p x :=
+exists.intro w ⟨h₁, h₂⟩
+
+attribute [recursor 4]
+theorem exists_unique.elim {α : Sort u} {p : α → Prop} {b : Prop}
+    (h₂ : ∃! x, p x) (h₁ : ∀ x, p x → (∀ y, p y → y = x) → b) : b :=
+exists.elim h₂ (λ w hw, h₁ w (and.left hw) (and.right hw))
+
+theorem exists_unique_of_exists_of_unique {α : Type u} {p : α → Prop}
+    (hex : ∃ x, p x) (hunique : ∀ y₁ y₂, p y₁ → p y₂ → y₁ = y₂) :  ∃! x, p x :=
+exists.elim hex (λ x px, exists_unique.intro x px (assume y, assume : p y, hunique y x this px))
+
+theorem exists_of_exists_unique {α : Sort u} {p : α → Prop} (h : ∃! x, p x) : ∃ x, p x :=
+exists.elim h (λ x hx, ⟨x, and.left hx⟩)
+
+theorem unique_of_exists_unique {α : Sort u} {p : α → Prop}
+    (h : ∃! x, p x) {y₁ y₂ : α} (py₁ : p y₁) (py₂ : p y₂) : y₁ = y₂ :=
+exists_unique.elim h
+  (assume x, assume : p x,
+    assume unique : ∀ y, p y → y = x,
+    show y₁ = y₂, from eq.trans (unique _ py₁) (eq.symm (unique _ py₂)))
+
+/- exists, forall, exists unique congruences -/
+@[congr] theorem forall_congr {α : Sort u} {p q : α → Prop} (h : ∀ a, (p a ↔ q a)) : (∀ a, p a) ↔ ∀ a, q a :=
+iff.intro (λ p a, iff.mp (h a) (p a)) (λ q a, iff.mpr (h a) (q a))
+
+theorem exists_imp_exists {α : Sort u} {p q : α → Prop} (h : ∀ a, (p a → q a)) (p : ∃ a, p a) : ∃ a, q a :=
+exists.elim p (λ a hp, ⟨a, h a hp⟩)
+
+@[congr] theorem exists_congr {α : Sort u} {p q : α → Prop} (h : ∀ a, (p a ↔ q a)) : (Exists p) ↔ ∃ a, q a :=
+iff.intro
+  (exists_imp_exists (λ a, iff.mp (h a)))
+  (exists_imp_exists (λ a, iff.mpr (h a)))
+
+@[congr] theorem exists_unique_congr {α : Sort u} {p₁ p₂ : α → Prop} (h : ∀ x, p₁ x ↔ p₂ x) : (exists_unique p₁) ↔ (∃! x, p₂ x) := --
+exists_congr (λ x, and_congr (h x) (forall_congr (λ y, imp_congr (h y) iff.rfl)))
+
+theorem forall_not_of_not_exists {α : Sort u} {p : α → Prop} : ¬(∃ x, p x) → (∀ x, ¬p x) :=
+λ hne x hp, hne ⟨x, hp⟩
+
+/- Decidable -/
+
+def decidable.to_bool (p : Prop) [h : decidable p] : bool :=
+decidable.cases_on h (λ h₁, bool.ff) (λ h₂, bool.tt)
+
+export decidable (is_true is_false to_bool)
+
+@[simp] theorem to_bool_true_eq_tt (h : decidable true) : @to_bool true h = tt :=
+decidable.cases_on h (λ h, false.elim (iff.mp not_true h)) (λ _, rfl)
+
+@[simp] theorem to_bool_false_eq_ff (h : decidable false) : @to_bool false h = ff :=
+decidable.cases_on h (λ h, rfl) (λ h, false.elim h)
+
+instance : decidable true :=
+is_true trivial
+
+instance : decidable false :=
+is_false not_false
+
+-- We use "dependent" if-then-else to be able to communicate the if-then-else condition
+-- to the branches
+@[inline] def dite (c : Prop) [h : decidable c] {α : Sort u} : (c → α) → (¬ c → α) → α :=
+λ t e, decidable.rec_on h e t
+
+/- if-then-else -/
+
+@[inline] def ite (c : Prop) [h : decidable c] {α : Sort u} (t e : α) : α :=
+decidable.rec_on h (λ hnc, e) (λ hc, t)
+
+namespace decidable
+variables {p q : Prop}
+
+def rec_on_true [h : decidable p] {h₁ : p → Sort u} {h₂ : ¬p → Sort u} (h₃ : p) (h₄ : h₁ h₃)
+    : (decidable.rec_on h h₂ h₁ : Sort u) :=
+decidable.rec_on h (λ h, false.rec _ (h h₃)) (λ h, h₄)
+
+def rec_on_false [h : decidable p] {h₁ : p → Sort u} {h₂ : ¬p → Sort u} (h₃ : ¬p) (h₄ : h₂ h₃)
+    : (decidable.rec_on h h₂ h₁ : Sort u) :=
+decidable.rec_on h (λ h, h₄) (λ h, false.rec _ (h₃ h))
+
+def by_cases {q : Sort u} [s : decidable p] (h1 : p → q) (h2 : ¬p → q) : q :=
+match s with
+| is_true h  := h1 h
+| is_false h := h2 h
+end
+
+theorem em (p : Prop) [decidable p] : p ∨ ¬p :=
+by_cases or.inl or.inr
+
+theorem by_contradiction [decidable p] (h : ¬p → false) : p :=
+by_cases id (λ np : ¬p, false.elim (h np))
+
+theorem of_not_not [decidable p] : ¬ ¬ p → p :=
+λ hnn, by_contradiction (λ hn, absurd hn hnn)
+
+theorem not_not_iff (p) [decidable p] : (¬ ¬ p) ↔ p :=
+iff.intro of_not_not not_not_intro
+
+theorem not_and_iff_or_not (p q : Prop) [d₁ : decidable p] [d₂ : decidable q] : ¬ (p ∧ q) ↔ ¬ p ∨ ¬ q :=
+iff.intro
+(λ h, match d₁ with
+      | is_true h₁  :=
+        match d₂ with
+        | is_true h₂  := absurd (and.intro h₁ h₂) h
+        | is_false h₂ := or.inr h₂
+        end
+      | is_false h₁ := or.inl h₁
+      end)
+(λ h ⟨hp, hq⟩, or.elim h (λ h, h hp) (λ h, h hq))
+
+theorem not_or_iff_and_not (p q) [d₁ : decidable p] [d₂ : decidable q] : ¬ (p ∨ q) ↔ ¬ p ∧ ¬ q :=
+iff.intro
+  (λ h, match d₁ with
+        | is_true h₁  := false.elim $ h (or.inl h₁)
+        | is_false h₁ :=
+          match d₂ with
+          | is_true h₂  := false.elim $ h (or.inr h₂)
+          | is_false h₂ := ⟨h₁, h₂⟩
+          end
+        end)
+  (λ ⟨np, nq⟩ h, or.elim h np nq)
+end decidable
+
+section
+variables {p q : Prop}
+def  decidable_of_decidable_of_iff (hp : decidable p) (h : p ↔ q) : decidable q :=
+if hp : p then is_true (iff.mp h hp)
+else is_false (iff.mp (not_iff_not_of_iff h) hp)
+
+def  decidable_of_decidable_of_eq (hp : decidable p) (h : p = q) : decidable q :=
+decidable_of_decidable_of_iff hp h.to_iff
+
+protected def or.by_cases [decidable p] [decidable q] {α : Sort u}
+                                 (h : p ∨ q) (h₁ : p → α) (h₂ : q → α) : α :=
+if hp : p then h₁ hp else
+  if hq : q then h₂ hq else
+    false.rec _ (or.elim h hp hq)
+end
+
+section
+variables {p q : Prop}
+
+instance [decidable p] [decidable q] : decidable (p ∧ q) :=
+if hp : p then
+  if hq : q then is_true ⟨hp, hq⟩
+  else is_false (assume h : p ∧ q, hq (and.right h))
+else is_false (assume h : p ∧ q, hp (and.left h))
+
+instance [decidable p] [decidable q] : decidable (p ∨ q) :=
+if hp : p then is_true (or.inl hp) else
+  if hq : q then is_true (or.inr hq) else
+    is_false (or.rec hp hq)
+
+instance [decidable p] : decidable (¬p) :=
+if hp : p then is_false (absurd hp) else is_true hp
+
+instance implies.decidable [decidable p] [decidable q] : decidable (p → q) :=
+if hp : p then
+  if hq : q then is_true (assume h, hq)
+  else is_false (assume h : p → q, absurd (h hp) hq)
+else is_true (assume h, absurd h hp)
+
+instance [decidable p] [decidable q] : decidable (p ↔ q) :=
+if hp : p then
+  if hq : q then is_true ⟨λ_, hq, λ_, hp⟩
+  else is_false $ λh, hq (h.1 hp)
+else
+  if hq : q then is_false $ λh, hp (h.2 hq)
+  else is_true $ ⟨λh, absurd h hp, λh, absurd h hq⟩
+
+instance [decidable p] [decidable q] : decidable (xor p q) :=
+if hp : p then
+  if hq : q then is_false (or.rec (λ ⟨_, h⟩, h hq : ¬(p ∧ ¬ q)) (λ ⟨_, h⟩, h hp : ¬(q ∧ ¬ p)))
+  else is_true $ or.inl ⟨hp, hq⟩
+else
+  if hq : q then is_true $ or.inr ⟨hq, hp⟩
+  else is_false (or.rec (λ ⟨h, _⟩, hp h : ¬(p ∧ ¬ q)) (λ ⟨h, _⟩, hq h : ¬(q ∧ ¬ p)))
+
+instance exists_prop_decidable {p} (P : p → Prop) [decidable p] [s : ∀ h, decidable (P h)] : decidable (∃ h, P h) :=
+if h : p then decidable_of_decidable_of_iff (s h)
+  ⟨λ h2, ⟨h, h2⟩, λ ⟨h', h2⟩, h2⟩ else is_false (mt (λ ⟨h, _⟩, h) h)
+
+instance forall_prop_decidable {p} (P : p → Prop)
+  [Dp : decidable p] [DP : ∀ h, decidable (P h)] : decidable (∀ h, P h) :=
+if h : p then decidable_of_decidable_of_iff (DP h)
+  ⟨λ h2 _, h2, λal, al h⟩ else is_true (λ h2, absurd h2 h)
+end
+
+instance {α : Sort u} [decidable_eq α] (a b : α) : decidable (a ≠ b) :=
+implies.decidable
+
+theorem bool.ff_ne_tt : ff = tt → false
+.
+
+def is_dec_eq {α : Sort u} (p : α → α → bool) : Prop   := ∀ ⦃x y : α⦄, p x y = tt → x = y
+def is_dec_refl {α : Sort u} (p : α → α → bool) : Prop := ∀ x, p x x = tt
+
+open decidable
+instance : decidable_eq bool
+| ff ff := is_true rfl
+| ff tt := is_false bool.ff_ne_tt
+| tt ff := is_false (ne.symm bool.ff_ne_tt)
+| tt tt := is_true rfl
+
+def decidable_eq_of_bool_pred {α : Sort u} {p : α → α → bool} (h₁ : is_dec_eq p) (h₂ : is_dec_refl p) : decidable_eq α :=
+assume x y : α,
+ if hp : p x y = tt then is_true (h₁ hp)
+ else is_false (assume hxy : x = y, absurd (h₂ y) (@eq.rec_on _ _ (λ z, ¬p z y = tt) _ hxy hp))
+
+theorem decidable_eq_inl_refl {α : Sort u} [h : decidable_eq α] (a : α) : h a a = is_true (eq.refl a) :=
+match (h a a) with
+| (is_true e)  := rfl
+| (is_false n) := absurd rfl n
+end
+
+theorem decidable_eq_inr_neg {α : Sort u} [h : decidable_eq α] {a b : α} : Π n : a ≠ b, h a b = is_false n :=
+assume n,
+match (h a b) with
+| (is_true e)   := absurd e n
+| (is_false n₁) := proof_irrel n n₁ ▸ eq.refl (is_false n)
+end
+
+
+
+theorem if_pos {c : Prop} [h : decidable c] (hc : c) {α : Sort u} {t e : α} : (ite c t e) = t :=
+match h with
+| (is_true  hc)  := rfl
+| (is_false hnc) := absurd hc hnc
+end
+
+theorem if_neg {c : Prop} [h : decidable c] (hnc : ¬c) {α : Sort u} {t e : α} : (ite c t e) = e :=
+match h with
+| (is_true hc)   := absurd hc hnc
+| (is_false hnc) := rfl
+end
+
+@[simp]
+theorem if_t_t (c : Prop) [h : decidable c] {α : Sort u} (t : α) : (ite c t t) = t :=
+match h with
+| (is_true hc)   := rfl
+| (is_false hnc) := rfl
+end
+
+theorem implies_of_if_pos {c t e : Prop} [decidable c] (h : ite c t e) : c → t :=
+assume hc, eq.rec_on (if_pos hc : ite c t e = t) h
+
+theorem implies_of_if_neg {c t e : Prop} [decidable c] (h : ite c t e) : ¬c → e :=
+assume hnc, eq.rec_on (if_neg hnc : ite c t e = e) h
+
+theorem if_ctx_congr {α : Sort u} {b c : Prop} [dec_b : decidable b] [dec_c : decidable c]
+                   {x y u v : α}
+                   (h_c : b ↔ c) (h_t : c → x = u) (h_e : ¬c → y = v) :
+        ite b x y = ite c u v :=
+match dec_b, dec_c with
+| (is_false h₁), (is_false h₂) := h_e h₂
+| (is_true h₁),  (is_true h₂)  := h_t h₂
+| (is_false h₁), (is_true h₂)  := absurd h₂ (iff.mp (not_iff_not_of_iff h_c) h₁)
+| (is_true h₁),  (is_false h₂) := absurd h₁ (iff.mpr (not_iff_not_of_iff h_c) h₂)
+end
+
+@[congr]
+theorem if_congr {α : Sort u} {b c : Prop} [dec_b : decidable b] [dec_c : decidable c]
+               {x y u v : α}
+               (h_c : b ↔ c) (h_t : x = u) (h_e : y = v) :
+        ite b x y = ite c u v :=
+@if_ctx_congr α b c dec_b dec_c x y u v h_c (λ h, h_t) (λ h, h_e)
+
+theorem if_ctx_simp_congr {α : Sort u} {b c : Prop} [dec_b : decidable b] {x y u v : α}
+                        (h_c : b ↔ c) (h_t : c → x = u) (h_e : ¬c → y = v) :
+        ite b x y = (@ite c (decidable_of_decidable_of_iff dec_b h_c) α u v) :=
+@if_ctx_congr α b c dec_b (decidable_of_decidable_of_iff dec_b h_c) x y u v h_c h_t h_e
+
+@[congr]
+theorem if_simp_congr {α : Sort u} {b c : Prop} [dec_b : decidable b] {x y u v : α}
+                    (h_c : b ↔ c) (h_t : x = u) (h_e : y = v) :
+        ite b x y = (@ite c (decidable_of_decidable_of_iff dec_b h_c) α u v) :=
+@if_ctx_simp_congr α b c dec_b x y u v h_c (λ h, h_t) (λ h, h_e)
+
+@[simp]
+theorem if_true {α : Sort u} {h : decidable true} (t e : α) : (@ite true h α t e) = t :=
+if_pos trivial
+
+@[simp]
+theorem if_false {α : Sort u} {h : decidable false} (t e : α) : (@ite false h α t e) = e :=
+if_neg not_false
+
+theorem if_ctx_congr_prop {b c x y u v : Prop} [dec_b : decidable b] [dec_c : decidable c]
+                      (h_c : b ↔ c) (h_t : c → (x ↔ u)) (h_e : ¬c → (y ↔ v)) :
+        ite b x y ↔ ite c u v :=
+match dec_b, dec_c with
+| (is_false h₁), (is_false h₂) := h_e h₂
+| (is_true h₁),  (is_true h₂)  := h_t h₂
+| (is_false h₁), (is_true h₂)  := absurd h₂ (iff.mp (not_iff_not_of_iff h_c) h₁)
+| (is_true h₁),  (is_false h₂) := absurd h₁ (iff.mpr (not_iff_not_of_iff h_c) h₂)
+end
+
+@[congr]
+theorem if_congr_prop {b c x y u v : Prop} [dec_b : decidable b] [dec_c : decidable c]
+                    (h_c : b ↔ c) (h_t : x ↔ u) (h_e : y ↔ v) :
+        ite b x y ↔ ite c u v :=
+if_ctx_congr_prop h_c (λ h, h_t) (λ h, h_e)
+
+theorem if_ctx_simp_congr_prop {b c x y u v : Prop} [dec_b : decidable b]
+                               (h_c : b ↔ c) (h_t : c → (x ↔ u)) (h_e : ¬c → (y ↔ v)) :
+        ite b x y ↔ (@ite c (decidable_of_decidable_of_iff dec_b h_c) Prop u v) :=
+@if_ctx_congr_prop b c x y u v dec_b (decidable_of_decidable_of_iff dec_b h_c) h_c h_t h_e
+
+@[congr]
+theorem if_simp_congr_prop {b c x y u v : Prop} [dec_b : decidable b]
+                           (h_c : b ↔ c) (h_t : x ↔ u) (h_e : y ↔ v) :
+        ite b x y ↔ (@ite c (decidable_of_decidable_of_iff dec_b h_c) Prop u v) :=
+@if_ctx_simp_congr_prop b c x y u v dec_b h_c (λ h, h_t) (λ h, h_e)
+
+@[simp] theorem dif_pos {c : Prop} [h : decidable c] (hc : c) {α : Sort u} {t : c → α} {e : ¬ c → α} : dite c t e = t hc :=
+match h with
+| (is_true hc)   := rfl
+| (is_false hnc) := absurd hc hnc
+end
+
+@[simp] theorem dif_neg {c : Prop} [h : decidable c] (hnc : ¬c) {α : Sort u} {t : c → α} {e : ¬ c → α} : dite c t e = e hnc :=
+match h with
+| (is_true hc)   := absurd hc hnc
+| (is_false hnc) := rfl
+end
+
+theorem dif_ctx_congr {α : Sort u} {b c : Prop} [dec_b : decidable b] [dec_c : decidable c]
+                    {x : b → α} {u : c → α} {y : ¬b → α} {v : ¬c → α}
+                    (h_c : b ↔ c)
+                    (h_t : ∀ (h : c),    x (iff.mpr h_c h)                      = u h)
+                    (h_e : ∀ (h : ¬c),   y (iff.mpr (not_iff_not_of_iff h_c) h) = v h) :
+        (@dite b dec_b α x y) = (@dite c dec_c α u v) :=
+match dec_b, dec_c with
+| (is_false h₁), (is_false h₂) := h_e h₂
+| (is_true h₁),  (is_true h₂)  := h_t h₂
+| (is_false h₁), (is_true h₂)  := absurd h₂ (iff.mp (not_iff_not_of_iff h_c) h₁)
+| (is_true h₁),  (is_false h₂) := absurd h₁ (iff.mpr (not_iff_not_of_iff h_c) h₂)
+end
+
+theorem dif_ctx_simp_congr {α : Sort u} {b c : Prop} [dec_b : decidable b]
+                         {x : b → α} {u : c → α} {y : ¬b → α} {v : ¬c → α}
+                         (h_c : b ↔ c)
+                         (h_t : ∀ (h : c),    x (iff.mpr h_c h)                      = u h)
+                         (h_e : ∀ (h : ¬c),   y (iff.mpr (not_iff_not_of_iff h_c) h) = v h) :
+        (@dite b dec_b α x y) = (@dite c (decidable_of_decidable_of_iff dec_b h_c) α u v) :=
+@dif_ctx_congr α b c dec_b (decidable_of_decidable_of_iff dec_b h_c) x u y v h_c h_t h_e
+
+-- Remark: dite and ite are "defally equal" when we ignore the proofs.
+theorem dif_eq_if (c : Prop) [h : decidable c] {α : Sort u} (t : α) (e : α) : dite c (λ h, t) (λ h, e) = ite c t e :=
+match h with
+| (is_true hc)   := rfl
+| (is_false hnc) := rfl
+end
+
+instance {c t e : Prop} [d_c : decidable c] [d_t : decidable t] [d_e : decidable e] : decidable (if c then t else e)  :=
+match d_c with
+| (is_true hc)  := d_t
+| (is_false hc) := d_e
+end
+
+instance {c : Prop} {t : c → Prop} {e : ¬c → Prop} [d_c : decidable c] [d_t : ∀ h, decidable (t h)] [d_e : ∀ h, decidable (e h)] : decidable (if h : c then t h else e h)  :=
+match d_c with
+| (is_true hc)  := d_t hc
+| (is_false hc) := d_e hc
+end
+
+def as_true (c : Prop) [decidable c] : Prop :=
+if c then true else false
+
+def as_false (c : Prop) [decidable c] : Prop :=
+if c then false else true
+
+def of_as_true {c : Prop} [h₁ : decidable c] (h₂ : as_true c) : c :=
+match h₁, h₂ with
+| (is_true h_c),  h₂ := h_c
+| (is_false h_c), h₂ := false.elim h₂
+end
+
 /-- Universe lifting operation -/
 structure {r s} ulift (α : Type s) : Type (max s r) :=
 up :: (down : α)
 
 namespace ulift
 /- Bijection between α and ulift.{v} α -/
-lemma up_down {α : Type u} : ∀ (b : ulift.{v} α), up (down b) = b
+theorem up_down {α : Type u} : ∀ (b : ulift.{v} α), up (down b) = b
 | (up a) := rfl
 
-lemma down_up {α : Type u} (a : α) : down (up.{v} a) = a := rfl
+theorem down_up {α : Type u} (a : α) : down (up.{v} a) = a := rfl
 end ulift
 
 /-- Universe lifting operation from Sort to Type -/
@@ -601,8 +1432,172 @@ up :: (down : α)
 
 namespace plift
 /- Bijection between α and plift α -/
-lemma up_down {α : Sort u} : ∀ (b : plift α), up (down b) = b
+theorem up_down {α : Sort u} : ∀ (b : plift α), up (down b) = b
 | (up a) := rfl
 
-lemma down_up {α : Sort u} (a : α) : down (up a) = a := rfl
+theorem down_up {α : Sort u} (a : α) : down (up a) = a := rfl
 end plift
+
+/- inhabited -/
+
+class inhabited (α : Sort u) :=
+(default : α)
+
+def default (α : Sort u) [inhabited α] : α :=
+inhabited.default α
+
+@[inline, irreducible] def arbitrary (α : Sort u) [inhabited α] : α :=
+default α
+
+instance prop.inhabited : inhabited Prop :=
+⟨true⟩
+
+instance fun.inhabited (α : Sort u) {β : Sort v} [h : inhabited β] : inhabited (α → β) :=
+inhabited.rec_on h (λ b, ⟨λ a, b⟩)
+
+instance pi.inhabited (α : Sort u) {β : α → Sort v} [Π x, inhabited (β x)] : inhabited (Π x, β x) :=
+⟨λ a, default (β a)⟩
+
+instance : inhabited bool := ⟨ff⟩
+
+instance : inhabited true := ⟨trivial⟩
+
+class inductive nonempty (α : Sort u) : Prop
+| intro (val : α) : nonempty
+
+protected def nonempty.elim {α : Sort u} {p : Prop} (h₁ : nonempty α) (h₂ : α → p) : p :=
+nonempty.rec h₂ h₁
+
+instance nonempty_of_inhabited {α : Sort u} [inhabited α] : nonempty α :=
+⟨default α⟩
+
+theorem nonempty_of_exists {α : Sort u} {p : α → Prop} : (∃ x, p x) → nonempty α
+| ⟨w, h⟩ := ⟨w⟩
+
+/- subsingleton -/
+
+class inductive subsingleton (α : Sort u) : Prop
+| intro (h : ∀ a b : α, a = b) : subsingleton
+
+protected def subsingleton.elim {α : Sort u} [h : subsingleton α] : ∀ (a b : α), a = b :=
+subsingleton.rec (λ p, p) h
+
+protected def subsingleton.helim {α β : Sort u} [h : subsingleton α] (h : α = β) : ∀ (a : α) (b : β), a == b :=
+eq.rec_on h (λ a b : α, heq_of_eq (subsingleton.elim a b))
+
+instance subsingleton_prop (p : Prop) : subsingleton p :=
+⟨λ a b, proof_irrel a b⟩
+
+instance (p : Prop) : subsingleton (decidable p) :=
+subsingleton.intro (λ d₁,
+  match d₁ with
+  | (is_true t₁) := (λ d₂,
+    match d₂ with
+    | (is_true t₂) := eq.rec_on (proof_irrel t₁ t₂) rfl
+    | (is_false f₂) := absurd t₁ f₂
+    end)
+  | (is_false f₁) := (λ d₂,
+    match d₂ with
+    | (is_true t₂) := absurd t₂ f₁
+    | (is_false f₂) := eq.rec_on (proof_irrel f₁ f₂) rfl
+    end)
+  end)
+
+protected theorem rec_subsingleton {p : Prop} [h : decidable p] {h₁ : p → Sort u} {h₂ : ¬p → Sort u}
+                                 [h₃ : Π (h : p), subsingleton (h₁ h)] [h₄ : Π (h : ¬p), subsingleton (h₂ h)]
+                                 : subsingleton (decidable.rec_on h h₂ h₁) :=
+match h with
+| (is_true h)  := h₃ h
+| (is_false h) := h₄ h
+end
+
+/- Equalities for rewriting let-expressions -/
+theorem let_value_eq {α : Sort u} {β : Sort v} {a₁ a₂ : α} (b : α → β) :
+                   a₁ = a₂ → (let x : α := a₁ in b x) = (let x : α := a₂ in b x) :=
+λ h, eq.rec_on h rfl
+
+theorem let_value_heq {α : Sort v} {β : α → Sort u} {a₁ a₂ : α} (b : Π x : α, β x) :
+                    a₁ = a₂ → (let x : α := a₁ in b x) == (let x : α := a₂ in b x) :=
+λ h, eq.rec_on h (heq.refl (b a₁))
+
+theorem let_body_eq {α : Sort v} {β : α → Sort u} (a : α) {b₁ b₂ : Π x : α, β x} :
+                  (∀ x, b₁ x = b₂ x) → (let x : α := a in b₁ x) = (let x : α := a in b₂ x) :=
+λ h, h a
+
+theorem let_eq {α : Sort v} {β : Sort u} {a₁ a₂ : α} {b₁ b₂ : α → β} :
+             a₁ = a₂ → (∀ x, b₁ x = b₂ x) → (let x : α := a₁ in b₁ x) = (let x : α := a₂ in b₂ x) :=
+λ h₁ h₂, eq.rec_on h₁ (h₂ a₁)
+
+section relation
+variables {α : Sort u} {β : Sort v} (r : β → β → Prop)
+local infix `≺`:50 := r
+
+def reflexive := ∀ x, x ≺ x
+
+def symmetric := ∀ ⦃x y⦄, x ≺ y → y ≺ x
+
+def transitive := ∀ ⦃x y z⦄, x ≺ y → y ≺ z → x ≺ z
+
+def equivalence := reflexive r ∧ symmetric r ∧ transitive r
+
+def total := ∀ x y, x ≺ y ∨ y ≺ x
+
+def mk_equivalence (rfl : reflexive r) (symm : symmetric r) (trans : transitive r) : equivalence r :=
+⟨rfl, symm, trans⟩
+
+def irreflexive := ∀ x, ¬ x ≺ x
+
+def anti_symmetric := ∀ ⦃x y⦄, x ≺ y → y ≺ x → x = y
+
+def empty_relation := λ a₁ a₂ : α, false
+
+def subrelation (q r : β → β → Prop) := ∀ ⦃x y⦄, q x y → r x y
+
+def inv_image (f : α → β) : α → α → Prop :=
+λ a₁ a₂, f a₁ ≺ f a₂
+
+theorem inv_image.trans (f : α → β) (h : transitive r) : transitive (inv_image r f) :=
+λ (a₁ a₂ a₃ : α) (h₁ : inv_image r f a₁ a₂) (h₂ : inv_image r f a₂ a₃), h h₁ h₂
+
+theorem inv_image.irreflexive (f : α → β) (h : irreflexive r) : irreflexive (inv_image r f) :=
+λ (a : α) (h₁ : inv_image r f a a), h (f a) h₁
+
+inductive tc {α : Sort u} (r : α → α → Prop) : α → α → Prop
+| base  : ∀ a b, r a b → tc a b
+| trans : ∀ a b c, tc a b → tc b c → tc a c
+end relation
+
+section binary
+variables {α : Type u} {β : Type v}
+variable f : α → α → α
+variable inv : α → α
+variable one : α
+local notation a * b := f a b
+local notation a ⁻¹  := inv a
+variable g : α → α → α
+local notation a + b := g a b
+
+def commutative        := ∀ a b, a * b = b * a
+def associative        := ∀ a b c, (a * b) * c = a * (b * c)
+def left_identity      := ∀ a, one * a = a
+def right_identity     := ∀ a, a * one = a
+def right_inverse      := ∀ a, a * a⁻¹ = one
+def left_cancelative   := ∀ a b c, a * b = a * c → b = c
+def right_cancelative  := ∀ a b c, a * b = c * b → a = c
+def left_distributive  := ∀ a b c, a * (b + c) = a * b + a * c
+def right_distributive := ∀ a b c, (a + b) * c = a * c + b * c
+def right_commutative (h : β → α → β) := ∀ b a₁ a₂, h (h b a₁) a₂ = h (h b a₂) a₁
+def left_commutative  (h : α → β → β) := ∀ a₁ a₂ b, h a₁ (h a₂ b) = h a₂ (h a₁ b)
+
+theorem left_comm : commutative f → associative f → left_commutative f :=
+assume hcomm hassoc, assume a b c, calc
+  a*(b*c) = (a*b)*c  : eq.symm (hassoc a b c)
+    ...   = (b*a)*c  : hcomm a b ▸ rfl
+    ...   = b*(a*c)  : hassoc b a c
+
+theorem right_comm : commutative f → associative f → right_commutative f :=
+assume hcomm hassoc, assume a b c, calc
+  (a*b)*c = a*(b*c) : hassoc a b c
+    ...   = a*(c*b) : hcomm b c ▸ rfl
+    ...   = (a*c)*b : eq.symm (hassoc a c b)
+end binary
