library/init/data/punit.lean
@@ -4,7 +4,7 @@ Released under Apache 2.0 license as described in the file LICENSE.
 Author: Leonardo de Moura
 -/
 prelude
-import init.logic
+import init.core
 
 lemma punit_eq (a b : punit) : a = b :=
 punit.rec_on a (punit.rec_on b rfl)
